basic_topology/OpenMap.lean
@@ -1,0 +1,40 @@
+import basic_topology.Topology
+import basic_topology.Continuity
+import basic_topology.Operations
+
+set_option linter.style.multiGoal false
+
+variable {X Y Z: Type*} {T₁: Family X} {T₂: Family Y} {T₃: Family Z}
+
+def Open_map (T₁: Family X) (T₂: Family Y) (f: X → Y): Prop :=
+  ∀V, Open T₁ V → Open T₂ (Set.image f V)
+
+theorem Open_map_iff_basis(ℬ T₁: Family X) (T₂: Family Y)(hT₁: IsTopology T₁)(hT₂: IsTopology T₂) (f:X→ Y)(hB: base T₁ ℬ ): Open_map T₁ T₂ f ↔ ∀B∈ℬ, Open T₂ (Set.image f B)  := by
+  constructor
+  intro h B hb
+  apply hB.1 at hb
+  apply h at hb
+  exact hb
+  rw[Open_map]
+  intro hb V hV
+  rw[open_iff_eq_interior]
+  ext y
+  constructor
+  intro hx
+  rw[interior_iff_basis_element (base_self T₂)]
+  simp at hx
+  obtain ⟨x,⟨hxV, hf ⟩ ⟩ :=hx
+  have : ∃B∈ ℬ , x∈ B ∧ B⊆ V := by
+    rw[open_iff_eq_interior,] at hV
+    rw[hV,interior_iff_basis_element hB] at hxV
+    exact hxV
+    exact hT₁
+  obtain ⟨B,⟨_,_,_ ⟩  ⟩ := this
+  use Set.image f B
+  repeat' (apply And.intro)
+  (expose_names; exact hb B left)
+  simp
+  use x
+  (expose_names; exact Set.image_mono right)
+  exact fun a ↦ neighborhood_mem a
+  exact hT₂
