basic_topology/Product.lean
@@ -1,8 +1,36 @@
 import basic_topology.Operations
 import basic_topology.Continuity
+import basic_topology.OpenMap
+
+
+set_option linter.style.multiGoal false
 
 variable {X Y: Type*}
-
+--Helper Theorem--
+theorem box_equal_prod_projections {A: Set X}{B: Set Y}: A.prod B = (Set.image Prod.fst (A.prod B)).prod (Set.image Prod.snd (A.prod B)) := by
+  refine Set.Subset.antisymm_iff.mpr ?_
+  constructor
+  · intro (x,y) hxy
+    have hx: x∈(Set.image Prod.fst (A.prod B)) := by
+      refine (Set.mem_image Prod.fst (A.prod B) x).mpr ?_
+      use (x,y)
+    have hy: y∈ (Set.image Prod.snd (A.prod B)) := by
+      refine (Set.mem_image Prod.snd (A.prod B) y).mpr ?_
+      use (x,y)
+    exact ⟨hx, hy⟩
+  · intro (x,y) hxy
+    rcases hxy with ⟨hx, hy⟩
+    rcases hx with ⟨p, hp_mem, hpx⟩
+    rcases hy with ⟨q, hq_mem, hqy⟩
+    simp at hpx
+    simp at hqy
+    have hA: x ∈ A := by
+      rw [← hpx]
+      exact hp_mem.1
+    have hB: y∈ B := by
+      rw[← hqy]
+      exact hq_mem.2
+    exact ⟨ hA,hB⟩
 -- Binary product topology
 def product_topology_basis (TX: Family X) (TY: Family Y): Set (Set (X × Y)) :=
   {UV | ∃ U V, U ∈ TX ∧ V ∈ TY ∧ UV = Set.prod U V}
@@ -48,56 +76,12 @@ theorem product_topology_product_open {TX: Family X} {TY: Family Y}
   Set.prod U V ∈ product_topology TX TY := by
   apply unions_mem
   exists U, V
-
--- Projections are open
-
-def proj₁ {X: Type u} {Y: Type v}: X × Y → X :=
-  fun p => p.1
-
-def pr₁ (p : X × Y) : X := p.1
-
-theorem product_topology_left_projection_open {TX: Family X} {TY: Family Y} (hTX: IsTopology TX) (hTY: IsTopology TY)
-  {U: Set (X × Y)} (hU: U ∈ product_topology TX TY) :
-  proj₁ '' U ∈ TX :=
-  sorry
-
-theorem product_topology_right_projection_open {TX: Family X} {TY: Family Y} (hTX: IsTopology TX) (hTY: IsTopology TY)
-  {U: Set (X × Y)} (hU: U ∈ product_topology TX TY) :
-  (fun x => x.2) '' U ∈ TY :=
-  sorry
-
 theorem boxes_base_product_topology {TX: Family X} {TY: Family Y}: base (product_topology TX TY) (product_topology_basis TX TY) := by
   rw [base_iff_unions]
   constructor
   · rw [product_topology]
     exact unions_sub (product_topology_basis TX TY)
   · rfl
-
-theorem box_equal_prod_projections {A: Set X}{B: Set Y}: A.prod B = (Set.image Prod.fst (A.prod B)).prod (Set.image Prod.snd (A.prod B)) := by
-  refine Set.Subset.antisymm_iff.mpr ?_
-  constructor
-  · intro (x,y) hxy
-    have hx: x∈(Set.image Prod.fst (A.prod B)) := by
-      refine (Set.mem_image Prod.fst (A.prod B) x).mpr ?_
-      use (x,y)
-    have hy: y∈ (Set.image Prod.snd (A.prod B)) := by
-      refine (Set.mem_image Prod.snd (A.prod B) y).mpr ?_
-      use (x,y)
-    exact ⟨hx, hy⟩
-  · intro (x,y) hxy
-    rcases hxy with ⟨hx, hy⟩
-    rcases hx with ⟨p, hp_mem, hpx⟩
-    rcases hy with ⟨q, hq_mem, hqy⟩
-    simp at hpx
-    simp at hqy
-    have hA: x ∈ A := by
-      rw [← hpx]
-      exact hp_mem.1
-    have hB: y∈ B := by
-      rw[← hqy]
-      exact hq_mem.2
-    exact ⟨ hA,hB⟩
-
 theorem boxes_subset_everywhere {TX: Family X} {TY: Family Y} (U: Set (X×Y))(hTX: IsTopology TX)(hTY: IsTopology TY)(hU: Open (product_topology TX TY) U): ∀x∈ U , ∃ A∈ product_topology_basis TX TY , x∈A ∧ A⊆ U := by
   intro x hx
   rw[ open_iff_eq_interior] at hU
@@ -106,12 +90,132 @@ theorem boxes_subset_everywhere {TX: Family X} {TY: Family Y} (U: Set (X×Y))(hT
     exact hx
   · exact product_topology_is_topology hTX hTY
 
+-- Projections Definitions
 
-
-theorem continuous_pr₁ (TX: Family X) (TY: Family Y)(hTx: IsTopology TX)(hTY: IsTopology TY) : Continuous (product_topology TX TY) (TX) (proj₁) := by
+def proj₁ {X: Type u} {Y: Type v}: X × Y → X :=
+  fun p => p.1
+def proj₂ {X: Type u} {Y: Type v}: X × Y → Y :=
+  fun p => p.2
+--Projections are continous--
+theorem continuous_pr₁ (TX: Family X) (TY: Family Y)(hTY: IsTopology TY) : Continuous (product_topology TX TY) (TX) (proj₁) := by
   unfold Continuous
   intro V hV
-  simp[Open]
   have hpr: proj₁⁻¹'V= V.prod (@Set.univ Y) := by
-    sorry
-  sorry
+    ext x
+    simp
+    rw[proj₁]
+    constructor
+    intro hx
+    have hx2: x.2∈ @Set.univ Y:= by trivial
+    exact ⟨ hx,hx2⟩
+    intro hx
+    exact hx.1
+  rw[hpr]
+  apply product_topology_product_open
+  exact hV
+  apply univ_open
+  exact hTY
+
+
+theorem continuous_pr₂ (TX: Family X) (TY: Family Y)(hTX: IsTopology TX) : Continuous (product_topology TX TY) (TY) (proj₂) := by
+  unfold Continuous
+  intro V hV
+  have hpr: proj₂⁻¹'V= (@Set.univ X).prod V := by
+    ext x
+    simp
+    rw[proj₂]
+    constructor
+    intro hx
+    have : x.2∈ @Set.univ Y:= by trivial
+    exact ⟨this , hx ⟩
+    intro hx
+    exact hx.2
+  rw[hpr]
+  apply product_topology_product_open
+  apply univ_open
+  exact hTX
+  exact hV
+
+
+--Projections are open maps
+theorem product_topology_left_projection_open {TX: Family X} {TY: Family Y} (hTX: IsTopology TX) (hTY: IsTopology TY): Open_map (product_topology TX TY) TX (proj₁)  := by
+  rw [Open_map_iff_basis (product_topology_basis TX TY)]
+  intro V hV
+  simp [product_topology_basis] at hV
+  obtain ⟨A,⟨hA,B,hB,hAB ⟩  ⟩:= hV
+  rcases Set.eq_empty_or_nonempty B with h1 | h2
+  have : V=∅ := by
+    rw[hAB]
+    by_contra h
+    push_neg at h
+    obtain ⟨x,hx ⟩:= h
+    have : B.Nonempty := by
+      refine Set.nonempty_def.mpr ?_
+      use x.2
+      exact hx.2
+    rw [Set.nonempty_iff_ne_empty] at this
+    exact this h1
+  rw[this]
+  simp
+  exact empty_open hTX
+  have : Set.image proj₁ V=A := by
+    ext x
+    simp
+    constructor
+    intro h
+    obtain ⟨a,⟨ b,hab,hproj⟩  ⟩ := h
+    simp [← hproj]
+    rw[hAB] at hab
+    exact hab.1
+    intro hx
+    obtain ⟨b,hb ⟩:= h2
+    use x, b
+    simp[proj₁]
+    rw[hAB]
+    exact ⟨hx,hb ⟩
+  rw[this]
+  exact hA
+  exact product_topology_is_topology hTX hTY
+  exact hTX
+  exact boxes_base_product_topology
+
+theorem product_topology_right_projection_open {TX: Family X} {TY: Family Y} (hTX: IsTopology TX) (hTY: IsTopology TY): Open_map (product_topology TX TY) TY (proj₂)  := by
+  rw [Open_map_iff_basis (product_topology_basis TX TY)]
+  intro V hV
+  simp [product_topology_basis] at hV
+  obtain ⟨A,⟨hA,B,hB,hAB ⟩  ⟩:= hV
+  rcases Set.eq_empty_or_nonempty A with h1 | h2
+  have : V=∅ := by
+    rw[hAB]
+    by_contra h
+    push_neg at h
+    obtain ⟨x,hx ⟩:= h
+    have : A.Nonempty := by
+      refine Set.nonempty_def.mpr ?_
+      use x.1
+      exact hx.1
+    rw [Set.nonempty_iff_ne_empty] at this
+    exact this h1
+  rw[this]
+  simp
+  exact empty_open hTY
+  have : Set.image proj₂ V=B := by
+    ext x
+    simp
+    constructor
+    intro h
+    obtain ⟨a,⟨ b,hab,hproj⟩  ⟩ := h
+    simp [← hproj]
+    rw[hAB] at hab
+    exact hab.2
+    intro hx
+    obtain ⟨b,hb ⟩:= h2
+    use b, x
+    simp[proj₂]
+    rw[hAB]
+    exact ⟨hb, hx ⟩
+  rw[this]
+  exact hB
+  exact product_topology_is_topology hTX hTY
+  exact hTY
+  exact boxes_base_product_topology
